mppa_k1c/Asmgenproof.v
@@ -17,18 +17,15 @@ Require Import Integers Floats AST Linking.
 Require Import Values Memory Events Globalenvs Smallstep.
 Require Import Op Locations Mach Conventions Asm Asmgen Machblockgen Asmblockgen.
 Require Import Machblockgenproof Asmblockgenproof PostpassSchedulingproof.
-Require Import Compopts.
 
 Local Open Scope linking_scope.
 
 Definition block_passes :=
       mkpass Machblockgenproof.match_prog
   ::: mkpass Asmblockgenproof.match_prog
-  ::: if Compopts.optim_postpass tt
-      then mkpass PostpassSchedulingproof.match_prog
-           ::: mkpass Asm.match_prog
-           ::: pass_nil _
-      else mkpass Asm.match_prog ::: pass_nil _.
+  ::: mkpass PostpassSchedulingproof.match_prog
+  ::: mkpass Asm.match_prog
+  ::: pass_nil _.
 
 Definition match_prog := pass_match (compose_passes block_passes).
 
@@ -39,16 +36,11 @@ Proof.
   unfold Asmgen.transf_program in H. apply bind_inversion in H. destruct H.
   inversion_clear H. apply bind_inversion in H1. destruct H1.
   inversion_clear H. inversion H2. remember (Machblockgen.transf_program p) as mbp.
-  unfold match_prog. simpl.
-  destruct (optim_postpass tt); simpl.
-  - exists mbp; split. apply Machblockgenproof.transf_program_match; auto.
-    exists x; split. apply Asmblockgenproof.transf_program_match; auto.
-    exists x0; split. apply PostpassSchedulingproof.transf_program_match; auto.
-    exists tp; split. apply Asm.transf_program_match; auto. auto.
-  - exists mbp; split. apply Machblockgenproof.transf_program_match; auto.
-    exists x0; split. apply Asmblockgenproof.transf_program_match; auto.
-    congruence.
-    exists tp; split. apply Asm.transf_program_match; auto. auto.
+  unfold match_prog; simpl.
+  exists mbp; split. apply Machblockgenproof.transf_program_match; auto.
+  exists x; split. apply Asmblockgenproof.transf_program_match; auto.
+  exists x0; split. apply PostpassSchedulingproof.transf_program_match; auto.
+  exists tp; split. apply Asm.transf_program_match; auto. auto.
 Qed.
 
 (** Return Address Offset *)
@@ -157,25 +149,15 @@ Let tge := Genv.globalenv tprog.
 Theorem transf_program_correct:
   forward_simulation (Mach.semantics return_address_offset prog) (Asm.semantics tprog).
 Proof.
-  unfold match_prog in TRANSF.
-  simpl in TRANSF.
-  inv TRANSF.
-  destruct (optim_postpass tt) in *.
-  - inv H. inv H1. inv H. inv H2. inv H. inv H3. inv H. inv H4.
-    eapply compose_forward_simulations. 
-    exploit Machblockgenproof.transf_program_correct; eauto.
-    unfold Machblockgenproof.inv_trans_rao. 
-    intros X; apply X.
-    eapply compose_forward_simulations. apply Asmblockgenproof.transf_program_correct; eauto.
-    eapply compose_forward_simulations. apply PostpassSchedulingproof.transf_program_correct; eauto.
-    apply Asm.transf_program_correct; eauto.
-  - inv H. inv H1. inv H. inv H2. inv H. inv H3.
-    eapply compose_forward_simulations. 
-    exploit Machblockgenproof.transf_program_correct; eauto.
-    unfold Machblockgenproof.inv_trans_rao. 
-    intros X; apply X.
-    eapply compose_forward_simulations. apply Asmblockgenproof.transf_program_correct; eauto.
-    apply Asm.transf_program_correct ; eauto.
+  unfold match_prog in TRANSF. simpl in TRANSF.
+  inv TRANSF. inv H. inv H1. inv H. inv H2. inv H. inv H3. inv H.
+  eapply compose_forward_simulations. 
+  exploit Machblockgenproof.transf_program_correct; eauto.
+  unfold Machblockgenproof.inv_trans_rao. 
+  intros X; apply X.
+  eapply compose_forward_simulations. apply Asmblockgenproof.transf_program_correct; eauto.
+  eapply compose_forward_simulations. apply PostpassSchedulingproof.transf_program_correct; eauto.
+  apply Asm.transf_program_correct. eauto.
 Qed.
 
 End PRESERVATION.
